RenamingSets/RenameAction/Basic.lean
@@ -10,4 +10,14 @@ lemma rename_one' : rename (1 : Ren 𝔸) = (id : X → X) := by
   ext a
   simp only [rename_one, id_eq]
 
+@[simp]
+lemma rename_discrete' [DiscreteRenameAction 𝔸 X] (σ : Ren 𝔸) : rename σ = (id : X → X) := by
+  ext
+  apply rename_discrete
+
+instance : DiscreteRenameAction[(default : RenameAction 𝔸 X)] := by
+  let : RenameAction 𝔸 X := default
+  constructor
+  simp only [RenameAction.default_rename, implies_true]
+
 end RenamingSets
